\documentclass[12pt]{article}
\usepackage{amsmath}
\usepackage{amssymb}
\usepackage{enumitem}
\usepackage{geometry}
\geometry{a4paper, margin=1in}

\begin{document}

\title{Problem Set 1}
\author{Liming Lin and Xinkai Xu}
\date{Sept.20, 2025}
\maketitle

\section*{Exercise 1}

\begin{enumerate}[label=\textbf{Question \arabic*:}, leftmargin=*, align=left]

    \item  
    \[
\max_{(c_t,k_{t+1})} \sum_{t=0}^{\infty} \beta^t \log(c_t) 
= \max_{(c_0,k_{t+1})} \Big\{ \log(c_0) + \sum_{t=1}^{\infty} \beta^t \log(c_t) \Big\}.
\]

\[
= \max_{(c_0,k_{t+1})} \; \log(c_0) + \beta \max_{(c_t,k_{t+1})} \sum_{t=0}^{\infty} \beta^{t}\log(c_{t+1}).
\]

Therefore,
\[
V(k_0) = \max_{(c_0,k_1)} \Big\{ \log(c_0) + \beta V(k_1) \Big\}.
\]

The recursive form of the problem is:
\[
V(k_t) = \max_{(c_t,k_{t+1})} \Big\{ \log(c_t) + \beta V(k_{t+1}) \Big\}.
\]

\noindent
\textbf{State variable:} $k_t$. \\
\textbf{Control variables:} $c_t, k_{t+1}$.\\
\textbf{Feasible set:} $\Gamma(k) = \{(c,k_{t+1}) : c_t + k_{t+1} \leq \theta k_t^\alpha, \; c_t,k_{t+1} \geq 0 \}$.


Using the resource constraint $c_t = \theta k_t^\alpha - k_{t+1}$, we can rewrite the Bellman equation as:
\[
V(k_t) = \max_{(c_t,k_{t+1})} \Big\{ \log(\theta k_t^\alpha - k_{t+1}) + \beta V(k_{t+1}) \Big\}.
\]

    \item
    a. FOC wrt to $k_{t+1}$:
\[
\frac{1}{\theta k_t^\alpha - k_{t+1}} = \beta V'(k_{t+1}),
\]
so
\[
\frac{1}{c_t} = \beta V'(k_{t+1}).
\]

b. Envelope theorem:
Consider $V'(k_t)$ at optimal value $k_{t+1}=g_k(k_t)$
\[
V'(k_{t}) = \frac{1}{\theta k_{t}^\alpha - k_{t+1}} \cdot \alpha \theta k_{t}^{\alpha-1}-\frac{1}{\theta k_{t}^\alpha - k_{t+1}} \cdot g'_k(k_t)+\beta V'(g_k(k_t)) \cdot g'_k(k_{t}).
\]

Thus
\[
V'(k_{t}) = \frac{1}{\theta k_t^\alpha - k_{t+1}}\alpha \theta k_t^{\alpha-1}+g'_k(k_t)(\beta V'(k_{t+1})-\frac{1}{\theta k_{t}^\alpha - k_{t+1}}).
\]
Given the FOC, the second term is zero, so
\[
V'(k_{t}) = \frac{1}{c_t}\alpha \theta k_t^{\alpha-1}.
\]
c. Combining the FOC and the envelope condition, we have
\[
\frac{1}{\theta k_t^\alpha - k_{t+1}} = \beta \frac{1}{c_{t+1}}\alpha \theta k_{t+1}^{\alpha-1},
\]
or simply
\[
u'(c_t) = \beta u'(c_{t+1}) f'(k_{t+1}).
\]

    \item  

a. Initial guess:
\[
V_0(k) = 0.
\]

Then
\[
V_1(k) = \max_{k_{t+1}} \log(\theta k_{t}^\alpha - k_{t+1}).
\]

Since there is no continuation value, the optimal choice is $k_{t+1}=0$, hence
\[
V_1(k) = \log(\theta k_{t}^\alpha).
\]


b. We then compute
\[
V_2(k) = \max_{k_{t+2}} \Big\{ \log(\theta k_{t+1}^\alpha - k_{t+2}) + \beta \log(\theta (k_{t+1})^\alpha) \Big\}.
\]

FOC wrt to $k_{t+2}$:
\[
-\frac{1}{\theta k_{t+1}^\alpha - k_{t+2}} + \frac{\beta \alpha}{k_{t+2}} = 0.
\]


So,
\[
\frac{1}{\theta k_{t+1}^\alpha - k_{t+2}} = \frac{\beta \alpha}{k_{t+2}}.
\]

This implies
\[
k_{t+2} = \beta \alpha \, \theta k_{t+1}^\alpha.
\]
or in general,
\[
k_{t+1} = \beta \alpha \, \theta k_{t}^\alpha.
\]

    \item 
   We guess the value function has the form
\[
V(k) = a_1 + a_2 \log k.
\]

The Bellman equation is
\[
V(k_t) = \max_{k_{t+1}} \Big\{ \log(\theta k_t^\alpha - k_{t+1}) + \beta V(k_{t+1}) \Big\}.
\]

So
\[
V(k_{t+1}) = a_1 + a_2 \log k_{t+1}
\]
and thus 
\[
V(k_t) = \max_{k_{t+1}} \Big\{ \log(\theta k_t^\alpha - k_{t+1}) + \beta (a_1 + a_2 \log k_{t+1}) \Big\}.
\]

FOC wrt to $k_{t+1}$:
\[
-\frac{1}{\theta k_t^\alpha - k_{t+1}} + \frac{\beta a_2}{k_{t+1}} = 0.
\]

Thus
\[
\theta k_t^\alpha - k_{t+1} = \frac{k_{t+1}}{\beta a_2}.
\]

Rearranging,
\[
k_{t+1} = \frac{\beta a_2}{1+\beta a_2} \theta k_t^\alpha.
\]

also,
\[
c_t = \theta k_t^\alpha - k_{t+1} = \frac{1}{1+\beta a_2} \theta k_t^\alpha.
\]

Back to the Bellman equation:
\[
V(k) = \log\left( \frac{\theta k^\alpha}{1+\beta a_2} \right)
+ \beta \Big( a_1 + a_2 \log\Big( \frac{\beta a_2}{1+\beta a_2}\theta k^\alpha \Big) \Big).
\]

\[
V(k) = \log(\theta k^\alpha) - \log(1+\beta a_2)
+ \beta a_1 + \beta a_2 \Big( \log\Big(\frac{\beta a_2}{1+\beta a_2}\Big) + \log(\theta k^\alpha) \Big).
\]
\[
= log(\theta) + \alpha \log(k) - \log(1+\beta a_2) + \beta a_1 + \beta a_2 \log\Big(\frac{\beta a_2}{1+\beta a_2}\Big) + \beta a_2 \log(\theta) + \alpha \beta a_2 \log(k).
\]


Looking for coefficients on $\log(k)$, we have
\[
a_2 = \alpha + \beta a_2 \alpha,
\]

which gives
\[
a_2 (1 - \alpha \beta) = \alpha,
\]

so
\[
a_2 = \frac{\alpha}{1-\alpha\beta}.
\]

similarly, looking for constant terms, we have
\[
a_1 = \log(\theta) - \log(1+\beta a_2) + \beta a_1 
+ \beta a_2 \left( \log\left(\frac{\beta a_2}{1+\beta a_2}\right) + \log \theta \right).
\]

Denote $C = \log(\theta) - \log(1+\beta a_2) + \beta a_2 \left( \log\left(\frac{\beta a_2}{1+\beta a_2}\right) + \log \theta \right)$, then
\[
a_1 = C + \beta a_1,
\]
so
\[
a_1  = \frac{C}{1-\beta}.
\]
Recall that $a_2 = \frac{\alpha}{1-\alpha\beta}$ and noticing that 
\[
1+\beta a_2 = \frac{1-\alpha\beta + \alpha\beta}{1-\alpha\beta} = \frac{1}{1-\alpha\beta},
\]
we have
\[
(1+\beta a_2) (1-\alpha\beta) = 1.
\]
Thus
\[
\beta a_2-\beta^2 a_2 \alpha = \alpha\beta,
\]
and then
\[\frac{\beta a_2} {1+\beta a_2} = \alpha\beta.
\]
Plugging these into $C$, we have
\[
C = \log(\theta(1-\alpha\beta)) + \beta \frac{\alpha}{1-\alpha\beta} \log(\alpha\beta\theta).
\]
    \item 
    Plug back into the function for $k_{t+1}$:
\[
k_{t+1} = \frac{\beta a_2}{1+\beta a_2} \theta k_t^\alpha = \alpha\beta \theta k_t^\alpha.
\]
similarly for $c_t$:
\[
c_t = \frac{1}{1+\beta a_2} \theta k_t^\alpha = (1-\alpha\beta) \theta k_t^\alpha.
\]

    \item 
Plug in the values of parameters:
\[
c_0 = (1-0.5*0.9) * 2 *1^{0.5}=1.1,
\]
\[
k_1 = 0.5*0.9*2*1^{0.5}=0.9,
\]
\[c_1 = (1-0.5*0.9) * 2 *0.9^{0.5}=1.043,
\]
\[
k_2 = 0.5*0.9*2*0.9^{0.5}=0.854,
\]
\[
c_2 = (1-0.5*0.9) * 2 *0.854^{0.5}=1.016.
\]

\end{enumerate}

\end{document}